Prove that if something has a beta-normal-form, then there is a lambda-term for computing the same normal-form.  Also really need to prove that if the computation comes to a normal-form, then the term does have one.  (And, thus, if the input doesn't have a normal-form, the computation will have to loop.)

examples/computability/lambda/churchDBScript.sml
@@ -1,4 +1,4 @@
-(* Church style encoding of de Bruijn terms, giving us 
+(* Church style encoding of de Bruijn terms, giving us
     "The Power of Reflection"
 *)
 
@@ -37,7 +37,7 @@ val NOT_IN_FV_ciDB = store_thm(
   METIS_TAC [FV_ciDB]);
 
 val is_abs_ciDB = Store_thm(
-  "is_abs_ciDB",  
+  "is_abs_ciDB",
   ``is_abs (ciDB t) ⇔ F``,
   Induct_on `t` THEN SRW_TAC [][ciDB_def]);
 
@@ -49,7 +49,7 @@ val bnf_ciDB = Store_thm(
 val ciDB_11 = Store_thm(
   "ciDB_11",
   ``(ciDB t1 = ciDB t2) = (t1 = t2)``,
-  Q.ID_SPEC_TAC `t2` THEN Induct_on `t1` THEN SRW_TAC [][ciDB_def] THEN 
+  Q.ID_SPEC_TAC `t2` THEN Induct_on `t1` THEN SRW_TAC [][ciDB_def] THEN
   Cases_on `t2` THEN SRW_TAC [][ciDB_def]);
 
 val cDB_def = Define`cDB t = LAM "v" (LAM "c" (LAM "a" (ciDB t)))`
@@ -74,54 +74,54 @@ val NOT_IN_SUB = prove(
 val cDB_thm = store_thm(
   "cDB_thm",
   ``cDB (dV i) @@ v @@ c @@ a == v @@ church i ∧
-    cDB (dAPP M N) @@ v @@ c @@ a == c @@ (cDB M @@ v @@ c @@ a) 
+    cDB (dAPP M N) @@ v @@ c @@ a == c @@ (cDB M @@ v @@ c @@ a)
                                        @@ (cDB N @@ v @@ c @@ a) ∧
     cDB (dABS M) @@ v @@ c @@ a == a @@ (cDB M @@ v @@ c @@ a)``,
   REPEAT CONJ_TAC THENL [
-    SIMP_TAC (bsrw_ss()) [cDB_def] THEN FRESH_TAC THEN 
-    SRW_TAC [][NOT_IN_FV_ciDB] THEN 
+    SIMP_TAC (bsrw_ss()) [cDB_def] THEN FRESH_TAC THEN
+    SRW_TAC [][NOT_IN_FV_ciDB] THEN
     ASM_SIMP_TAC (bsrw_ss()) [ciDB_def, tpm_fresh],
 
-    SIMP_TAC (srw_ss()) [cDB_def, ciDB_def] THEN 
-    Q_TAC (NEW_TAC "aa") `{"v"; "c"; "a"} ∪ FV v ∪ FV c ∪ FV a` THEN 
-    `(LAM "a" (VAR "c" @@ ciDB M @@ ciDB N) = 
+    SIMP_TAC (srw_ss()) [cDB_def, ciDB_def] THEN
+    Q_TAC (NEW_TAC "aa") `{"v"; "c"; "a"} ∪ FV v ∪ FV c ∪ FV a` THEN
+    `(LAM "a" (VAR "c" @@ ciDB M @@ ciDB N) =
         LAM aa (VAR "c" @@ [VAR aa/"a"](ciDB M) @@ [VAR aa/"a"](ciDB N))) ∧
      (LAM "a" (ciDB M) = LAM aa ([VAR aa/"a"](ciDB M))) ∧
      (LAM "a" (ciDB N) = LAM aa ([VAR aa/"a"](ciDB N)))`
-       by SRW_TAC [][LAM_eq_thm, NOT_IN_SUB, fresh_tpm_subst, 
-                     lemma15b, NOT_IN_FV_ciDB] THEN 
-    NTAC 3 (POP_ASSUM SUBST1_TAC) THEN 
+       by SRW_TAC [][LAM_eq_thm, NOT_IN_SUB, fresh_tpm_subst,
+                     lemma15b, NOT_IN_FV_ciDB] THEN
+    NTAC 3 (POP_ASSUM SUBST1_TAC) THEN
 
-    Q_TAC (NEW_TAC "cc") `{"v"; "c"; "a"; aa} ∪ FV v ∪ FV c ∪ FV a` THEN 
-    `(LAM "c" (LAM aa (VAR "c" @@ [VAR aa/"a"](ciDB M) 
-                               @@ [VAR aa/"a"](ciDB N))) = 
-        LAM cc (LAM aa (VAR cc @@ [VAR cc/"c"]([VAR aa/"a"](ciDB M)) 
+    Q_TAC (NEW_TAC "cc") `{"v"; "c"; "a"; aa} ∪ FV v ∪ FV c ∪ FV a` THEN
+    `(LAM "c" (LAM aa (VAR "c" @@ [VAR aa/"a"](ciDB M)
+                               @@ [VAR aa/"a"](ciDB N))) =
+        LAM cc (LAM aa (VAR cc @@ [VAR cc/"c"]([VAR aa/"a"](ciDB M))
                                @@ [VAR cc/"c"]([VAR aa/"a"](ciDB N))))) ∧
-     (LAM "c" (LAM aa ([VAR aa/"a"] (ciDB M))) = 
+     (LAM "c" (LAM aa ([VAR aa/"a"] (ciDB M))) =
         LAM cc (LAM aa ([VAR cc/"c"]([VAR aa/"a"] (ciDB M))))) ∧
-     (LAM "c" (LAM aa ([VAR aa/"a"] (ciDB N))) = 
+     (LAM "c" (LAM aa ([VAR aa/"a"] (ciDB N))) =
         LAM cc (LAM aa ([VAR cc/"c"]([VAR aa/"a"] (ciDB N)))))`
-       by SRW_TAC [][LAM_eq_thm, NOT_IN_SUB, fresh_tpm_subst, 
-                     lemma15b, NOT_IN_FV_ciDB] THEN 
-    NTAC 3 (POP_ASSUM SUBST1_TAC) THEN 
+       by SRW_TAC [][LAM_eq_thm, NOT_IN_SUB, fresh_tpm_subst,
+                     lemma15b, NOT_IN_FV_ciDB] THEN
+    NTAC 3 (POP_ASSUM SUBST1_TAC) THEN
     ASM_SIMP_TAC (bsrw_ss()) [],
 
-    SIMP_TAC (srw_ss()) [cDB_def, ciDB_def] THEN 
-    Q_TAC (NEW_TAC "aa") `{"v"; "c"; "a"} ∪ FV v ∪ FV c ∪ FV a` THEN 
+    SIMP_TAC (srw_ss()) [cDB_def, ciDB_def] THEN
+    Q_TAC (NEW_TAC "aa") `{"v"; "c"; "a"} ∪ FV v ∪ FV c ∪ FV a` THEN
     `(LAM "a" (VAR "a" @@ ciDB M) = LAM aa (VAR aa @@ [VAR aa/"a"](ciDB M))) ∧
      (LAM "a" (ciDB M) = LAM aa ([VAR aa/"a"](ciDB M)))`
-       by SRW_TAC [][LAM_eq_thm, NOT_IN_SUB, fresh_tpm_subst, 
-                     lemma15b, NOT_IN_FV_ciDB] THEN 
-    NTAC 2 (POP_ASSUM SUBST1_TAC) THEN 
+       by SRW_TAC [][LAM_eq_thm, NOT_IN_SUB, fresh_tpm_subst,
+                     lemma15b, NOT_IN_FV_ciDB] THEN
+    NTAC 2 (POP_ASSUM SUBST1_TAC) THEN
 
-    Q_TAC (NEW_TAC "cc") `{"v"; "c"; "a"; aa} ∪ FV v ∪ FV c ∪ FV a` THEN 
-    `(LAM "c" (LAM aa (VAR aa @@ [VAR aa/"a"](ciDB M))) = 
+    Q_TAC (NEW_TAC "cc") `{"v"; "c"; "a"; aa} ∪ FV v ∪ FV c ∪ FV a` THEN
+    `(LAM "c" (LAM aa (VAR aa @@ [VAR aa/"a"](ciDB M))) =
         LAM cc (LAM aa (VAR aa @@ [VAR cc/"c"]([VAR aa/"a"](ciDB M))))) ∧
-     (LAM "c" (LAM aa ([VAR aa/"a"](ciDB M))) = 
+     (LAM "c" (LAM aa ([VAR aa/"a"](ciDB M))) =
         LAM cc (LAM aa ([VAR cc/"c"]([VAR aa/"a"] (ciDB M)))))`
-       by SRW_TAC [][LAM_eq_thm, NOT_IN_SUB, fresh_tpm_subst, 
-                     lemma15b, NOT_IN_FV_ciDB] THEN 
-    NTAC 2 (POP_ASSUM SUBST1_TAC) THEN 
+       by SRW_TAC [][LAM_eq_thm, NOT_IN_SUB, fresh_tpm_subst,
+                     lemma15b, NOT_IN_FV_ciDB] THEN
+    NTAC 2 (POP_ASSUM SUBST1_TAC) THEN
     ASM_SIMP_TAC (bsrw_ss()) []
   ]);
 
@@ -134,29 +134,29 @@ dfv (dABS t) = λi. dfv t (i + 1)
 
 val cdFV_def = Define`
   cdFV = LAM "v" (LAM "t"
-           (VAR "t" @@ 
-              (LAM "j" (LAM "i" (ceqnat @@ VAR "i" @@ VAR "j"))) @@ 
-              (LAM "r1" (LAM "r2" (LAM "i" (cor @@ (VAR "r1" @@ VAR "i") @@ 
+           (VAR "t" @@
+              (LAM "j" (LAM "i" (ceqnat @@ VAR "i" @@ VAR "j"))) @@
+              (LAM "r1" (LAM "r2" (LAM "i" (cor @@ (VAR "r1" @@ VAR "i") @@
                                                    (VAR "r2" @@ VAR "i"))))) @@
-              (LAM "r" (LAM "i" (VAR "r" @@ (csuc @@ (VAR "i"))))) @@ 
+              (LAM "r" (LAM "i" (VAR "r" @@ (csuc @@ (VAR "i"))))) @@
               (VAR "v")))
 `;
 
 val FV_cdFV = Store_thm(
   "FV_cdFV",
   ``FV cdFV = {}``,
-  SRW_TAC [][cdFV_def, FV_EMPTY]); 
+  SRW_TAC [][cdFV_def, FV_EMPTY]);
 val cdFV_behaviour = store_thm(
   "cdFV_behaviour",
   ``∀i. cdFV @@ church i @@ cDB t -n->* cB (i ∈ dFV t)``,
-  SIMP_TAC (bsrw_ss()) [cdFV_def] THEN 
-  Induct_on `t` THEN 
-  ASM_SIMP_TAC (bsrw_ss()) [cDB_thm, ceqnat_behaviour, 
-                            cor_behaviour, csuc_behaviour, 
+  SIMP_TAC (bsrw_ss()) [cdFV_def] THEN
+  Induct_on `t` THEN
+  ASM_SIMP_TAC (bsrw_ss()) [cDB_thm, ceqnat_behaviour,
+                            cor_behaviour, csuc_behaviour,
                             arithmeticTheory.ADD1] THEN
   SRW_TAC [][EQ_SYM_EQ]);
 
-(* ---------------------------------------------------------------------- 
+(* ----------------------------------------------------------------------
     The constructors of the type in the λ-calculus
    ---------------------------------------------------------------------- *)
 
@@ -174,8 +174,8 @@ val cdV_behaviour = store_thm(
   SIMP_TAC (bsrw_ss()) [cdV_def, cDB_def, ciDB_def]);
 
 val cdAPP_def = Define`
-  cdAPP = LAM "M" (LAM "N" (LAM "v" (LAM "c" (LAM "a" 
-            (VAR "c" @@ (VAR "M" @@ VAR "v" @@ VAR "c" @@ VAR "a") @@ 
+  cdAPP = LAM "M" (LAM "N" (LAM "v" (LAM "c" (LAM "a"
+            (VAR "c" @@ (VAR "M" @@ VAR "v" @@ VAR "c" @@ VAR "a") @@
                         (VAR "N" @@ VAR "v" @@ VAR "c" @@ VAR "a"))))))
 `
 val FV_cdAPP = Store_thm(
@@ -191,11 +191,11 @@ val is_abs_cdAPP = Store_thm(
 val cdAPP_behaviour = store_thm(
   "cdAPP_behaviour",
   ``cdAPP @@ cDB M @@ cDB N -n->* cDB (dAPP M N)``,
-  SIMP_TAC (bsrw_ss()) [cdAPP_def] THEN 
+  SIMP_TAC (bsrw_ss()) [cdAPP_def] THEN
   SIMP_TAC (bsrw_ss()) [cDB_def, ciDB_def]);
 
 val cdABS_def = Define`
-  cdABS = LAM "M" (LAM "v" (LAM "c" (LAM "a" 
+  cdABS = LAM "M" (LAM "v" (LAM "c" (LAM "a"
             (VAR "a" @@ (VAR "M" @@ VAR "v" @@ VAR "c" @@ VAR "a")))))
 `;
 val FV_cdABS = Store_thm(
@@ -210,10 +210,10 @@ val is_abs_cdABS = Store_thm(
 val cdABS_behaviour = store_thm(
   "cdABS_behaviour",
   ``cdABS @@ cDB M -n->* cDB (dABS M)``,
-  SIMP_TAC (bsrw_ss()) [cdABS_def] THEN 
+  SIMP_TAC (bsrw_ss()) [cdABS_def] THEN
   SIMP_TAC (bsrw_ss()) [cDB_def, ciDB_def]);
 
-(* 
+(*
 val lift_def = Define`
   (lift (dV i) k = if i < k then dV i else dV (i + 1)) /\
   (lift (dAPP s t) k = dAPP (lift s k) (lift t k)) /\
@@ -222,12 +222,12 @@ val lift_def = Define`
 *)
 
 val clift_def = Define`
-  clift = 
+  clift =
   LAM "t"
-    (VAR "t" 
-         @@ (LAM "i" (LAM "k" (cless @@ VAR "i" @@ VAR "k" 
+    (VAR "t"
+         @@ (LAM "i" (LAM "k" (cless @@ VAR "i" @@ VAR "k"
                                      @@ (cdV @@ VAR "i")
-                                     @@ (cdV @@ (csuc @@ VAR "i"))))) 
+                                     @@ (cdV @@ (csuc @@ VAR "i")))))
          @@ (LAM "r1" (LAM "r2" (LAM "k"
                (cdAPP @@ (VAR "r1" @@ VAR "k") @@ (VAR "r2" @@ VAR "k")))))
          @@ (LAM "r" (LAM "k"
@@ -244,19 +244,19 @@ val is_abs_clift = Store_thm(
   SRW_TAC [][clift_def]);
 
 val clift_behaviour = store_thm(
-  "clift_behaviour",  
+  "clift_behaviour",
   ``clift @@ cDB M @@ church k -n->* cDB (lift M k)``,
-  SIMP_TAC (bsrw_ss()) [clift_def] THEN 
+  SIMP_TAC (bsrw_ss()) [clift_def] THEN
   Q.ID_SPEC_TAC `k` THEN Induct_on `M` THEN
-  ASM_SIMP_TAC (bsrw_ss()) 
-               [cDB_thm, cless_behaviour, cdV_behaviour, 
-                csuc_behaviour, cdAPP_behaviour, cdABS_behaviour, 
-                arithmeticTheory.ADD1] THEN 
-  SRW_TAC [][] THEN 
+  ASM_SIMP_TAC (bsrw_ss())
+               [cDB_thm, cless_behaviour, cdV_behaviour,
+                csuc_behaviour, cdAPP_behaviour, cdABS_behaviour,
+                arithmeticTheory.ADD1] THEN
+  SRW_TAC [][] THEN
   SIMP_TAC (bsrw_ss()) [cB_behaviour]);
 
 (* ----------------------------------------------------------------------
-    substitution 
+    substitution
    ---------------------------------------------------------------------- *)
 
 (* (∀s k i. sub s k (dV i) = if i = k then s else dV i) ∧
@@ -264,38 +264,38 @@ val clift_behaviour = store_thm(
    ∀s k t. sub s k (dABS t) = dABS (sub (lift s 0) (k + 1) t) *)
 
 val csub_def = Define`
-  csub = 
+  csub =
   LAM "s" (LAM "k" (LAM "t"
-    (VAR "t" 
-      @@ (LAM "i" (LAM "ss" (LAM "kk" 
+    (VAR "t"
+      @@ (LAM "i" (LAM "ss" (LAM "kk"
            (ceqnat @@ VAR "i" @@ VAR "kk" @@ VAR "ss" @@ (cdV @@ VAR "i")))))
       @@ (LAM "r1" (LAM "r2" (LAM "ss" (LAM "kk"
-           (cdAPP @@ (VAR "r1" @@ VAR "ss" @@ VAR "kk") 
+           (cdAPP @@ (VAR "r1" @@ VAR "ss" @@ VAR "kk")
                   @@ (VAR "r2" @@ VAR "ss" @@ VAR "kk"))))))
       @@ (LAM "r" (LAM "ss" (LAM "kk"
-           (cdABS @@ (VAR "r" @@ (clift @@ VAR "ss" @@ church 0) 
+           (cdABS @@ (VAR "r" @@ (clift @@ VAR "ss" @@ church 0)
                               @@ (csuc @@ VAR "kk"))))))
       @@ VAR "s" @@ VAR "k")))
 `;
 val FV_csub = Store_thm(
   "FV_csub",
   ``FV csub = {}``,
-  SRW_TAC [][csub_def, FV_EMPTY]); 
-           
+  SRW_TAC [][csub_def, FV_EMPTY]);
+
 val csub_behaviour = store_thm(
   "csub_behaviour",
   ``csub @@ cDB s @@ church k @@ cDB t -n->* cDB (sub s k t)``,
-  SIMP_TAC (bsrw_ss()) [csub_def] THEN 
-  MAP_EVERY Q.ID_SPEC_TAC [`s`, `k`] THEN Induct_on `t` THEN 
-  ASM_SIMP_TAC (bsrw_ss()) [cDB_thm, ceqnat_behaviour, cdV_behaviour, 
-                            cdAPP_behaviour, cdABS_behaviour, 
-                            csuc_behaviour, arithmeticTheory.ADD1, 
+  SIMP_TAC (bsrw_ss()) [csub_def] THEN
+  MAP_EVERY Q.ID_SPEC_TAC [`s`, `k`] THEN Induct_on `t` THEN
+  ASM_SIMP_TAC (bsrw_ss()) [cDB_thm, ceqnat_behaviour, cdV_behaviour,
+                            cdAPP_behaviour, cdABS_behaviour,
+                            csuc_behaviour, arithmeticTheory.ADD1,
                             clift_behaviour] THEN
   SRW_TAC [][] THEN SIMP_TAC (bsrw_ss()) [cB_behaviour])
 
 val cdLAM_def = Define`
   cdLAM = LAM "v" (LAM "body"
-            (cdABS @@ (csub @@ (cdV @@ church 0) 
+            (cdABS @@ (csub @@ (cdV @@ church 0)
                             @@ (cplus @@ (VAR "v") @@ church 1)
                             @@ (clift @@ (VAR "body") @@ church 0))))
 `;
@@ -308,8 +308,8 @@ val FV_cdLAM = Store_thm(
 val cdLAM_behaviour = store_thm(
   "cdLAM_behaviour",
   ``cdLAM @@ church i @@ cDB t -n->* cDB (dLAM i t)``,
-  SIMP_TAC (bsrw_ss()) [cdLAM_def, cdV_behaviour, cplus_behaviour, 
-                        clift_behaviour, csub_behaviour, cdABS_behaviour, 
+  SIMP_TAC (bsrw_ss()) [cdLAM_def, cdV_behaviour, cplus_behaviour,
+                        clift_behaviour, csub_behaviour, cdABS_behaviour,
                         dLAM_def]);
 
 (* ----------------------------------------------------------------------
@@ -319,48 +319,48 @@ val cdLAM_behaviour = store_thm(
 val B_I_uncond = store_thm(
   "B_I_uncond",
   ``v ∉ FV M ∧ v ∈ FV N ⇒ (LAM v (M @@ N) == B @@ M @@ (LAM v N))``,
-  STRIP_TAC THEN 
-  ASM_SIMP_TAC (bsrw_ss()) [chap2Theory.B_def] THEN 
-  REWRITE_TAC [chap2Theory.S_def] THEN 
-  Q_TAC (NEW_TAC "z") `{"x"; "y"; "z"} ∪ FV M ∪ FV N` THEN 
-  `LAM "z" (VAR "x" @@ VAR "z" @@ (VAR "y" @@ VAR "z")) = 
+  STRIP_TAC THEN
+  ASM_SIMP_TAC (bsrw_ss()) [chap2Theory.B_def] THEN
+  REWRITE_TAC [chap2Theory.S_def] THEN
+  Q_TAC (NEW_TAC "z") `{"x"; "y"; "z"} ∪ FV M ∪ FV N` THEN
+  `LAM "z" (VAR "x" @@ VAR "z" @@ (VAR "y" @@ VAR "z")) =
    LAM z (VAR "x" @@ VAR z @@ (VAR "y" @@ VAR z))`
-     by SRW_TAC [][LAM_eq_thm] THEN 
-  POP_ASSUM SUBST1_TAC THEN 
-  Q_TAC (NEW_TAC "y") `{"x"; "y"; z} ∪ FV M ∪ FV N` THEN 
+     by SRW_TAC [][LAM_eq_thm] THEN
+  POP_ASSUM SUBST1_TAC THEN
+  Q_TAC (NEW_TAC "y") `{"x"; "y"; z} ∪ FV M ∪ FV N` THEN
   `LAM "y" (LAM z (VAR "x" @@ VAR z @@ (VAR "y" @@ VAR z))) =
    LAM y (LAM z (VAR "x" @@ VAR z @@ (VAR y @@ VAR z)))`
-     by SRW_TAC [][LAM_eq_thm] THEN 
-  POP_ASSUM SUBST1_TAC THEN 
-  ASM_SIMP_TAC (bsrw_ss()) [] THEN 
-  `∀x y. (x = y) ⇒ (x == y)` by SRW_TAC [][] THEN POP_ASSUM MATCH_MP_TAC THEN 
-  SRW_TAC [boolSimps.CONJ_ss][LAM_eq_thm, tpm_fresh, NOT_IN_SUB] THEN 
+     by SRW_TAC [][LAM_eq_thm] THEN
+  POP_ASSUM SUBST1_TAC THEN
+  ASM_SIMP_TAC (bsrw_ss()) [] THEN
+  `∀x y. (x = y) ⇒ (x == y)` by SRW_TAC [][] THEN POP_ASSUM MATCH_MP_TAC THEN
+  SRW_TAC [boolSimps.CONJ_ss][LAM_eq_thm, tpm_fresh, NOT_IN_SUB] THEN
   SRW_TAC [][GSYM fresh_tpm_subst, tpm_flip_args]);
 
 val B_I = store_thm(
   "B_I",
-  ``v ∉ FV M ∧ v ∈ FV N ∧ N ≠ VAR v ⇒ 
+  ``v ∉ FV M ∧ v ∈ FV N ∧ N ≠ VAR v ⇒
       (LAM v (M @@ N) == B @@ M @@ (LAM v N))``,
   METIS_TAC [B_I_uncond]);
 
 val C_I = store_thm(
   "C_I",
   ``v ∈ FV M ∧ v ∉ FV N ⇒ LAM v (M @@ N) == C @@ (LAM v M) @@ N``,
-  STRIP_TAC THEN ASM_SIMP_TAC (bsrw_ss()) [chap2Theory.C_def] THEN 
-  REWRITE_TAC [chap2Theory.S_def] THEN 
-  Q_TAC (NEW_TAC "z") `{"x"; "y"; "z"} ∪ FV M ∪ FV N` THEN 
-  `LAM "z" (VAR "x" @@ VAR "z" @@ (VAR "y" @@ VAR "z")) = 
+  STRIP_TAC THEN ASM_SIMP_TAC (bsrw_ss()) [chap2Theory.C_def] THEN
+  REWRITE_TAC [chap2Theory.S_def] THEN
+  Q_TAC (NEW_TAC "z") `{"x"; "y"; "z"} ∪ FV M ∪ FV N` THEN
+  `LAM "z" (VAR "x" @@ VAR "z" @@ (VAR "y" @@ VAR "z")) =
    LAM z (VAR "x" @@ VAR z @@ (VAR "y" @@ VAR z))`
-     by SRW_TAC [][LAM_eq_thm] THEN 
-  POP_ASSUM SUBST1_TAC THEN 
-  Q_TAC (NEW_TAC "y") `{"x"; "y"; z} ∪ FV M ∪ FV N` THEN 
+     by SRW_TAC [][LAM_eq_thm] THEN
+  POP_ASSUM SUBST1_TAC THEN
+  Q_TAC (NEW_TAC "y") `{"x"; "y"; z} ∪ FV M ∪ FV N` THEN
   `LAM "y" (LAM z (VAR "x" @@ VAR z @@ (VAR "y" @@ VAR z))) =
    LAM y (LAM z (VAR "x" @@ VAR z @@ (VAR y @@ VAR z)))`
-     by SRW_TAC [][LAM_eq_thm] THEN 
-  POP_ASSUM SUBST1_TAC THEN 
-  ASM_SIMP_TAC (bsrw_ss()) [NOT_IN_SUB] THEN 
-  `∀x y. (x = y) ⇒ (x == y)` by SRW_TAC [][] THEN POP_ASSUM MATCH_MP_TAC THEN 
-  SRW_TAC [boolSimps.CONJ_ss][LAM_eq_thm, tpm_fresh, NOT_IN_SUB] THEN 
+     by SRW_TAC [][LAM_eq_thm] THEN
+  POP_ASSUM SUBST1_TAC THEN
+  ASM_SIMP_TAC (bsrw_ss()) [NOT_IN_SUB] THEN
+  `∀x y. (x = y) ⇒ (x == y)` by SRW_TAC [][] THEN POP_ASSUM MATCH_MP_TAC THEN
+  SRW_TAC [boolSimps.CONJ_ss][LAM_eq_thm, tpm_fresh, NOT_IN_SUB] THEN
   SRW_TAC [][GSYM fresh_tpm_subst, tpm_flip_args]);
 
 val I_I = store_thm(
@@ -369,69 +369,69 @@ val I_I = store_thm(
   SIMP_TAC (srw_ss()) [LAM_eq_thm, chap2Theory.I_def]);
 
 val K_I = store_thm(
-  "K_I", 
+  "K_I",
   ``v ∉ FV M ⇒ (LAM v M == K @@ M)``,
-  STRIP_TAC THEN REWRITE_TAC [chap2Theory.K_def] THEN 
-  Q_TAC (NEW_TAC "y") `{"x"; "y"} ∪ FV M` THEN 
-  `LAM "y" (VAR "x") = LAM y (VAR "x")` by SRW_TAC [][LAM_eq_thm] THEN 
-  POP_ASSUM SUBST1_TAC THEN 
-  ASM_SIMP_TAC (bsrw_ss()) [] THEN 
-  `∀x y. (x = y) ⇒ (x == y)` by SRW_TAC [][] THEN POP_ASSUM MATCH_MP_TAC THEN 
+  STRIP_TAC THEN REWRITE_TAC [chap2Theory.K_def] THEN
+  Q_TAC (NEW_TAC "y") `{"x"; "y"} ∪ FV M` THEN
+  `LAM "y" (VAR "x") = LAM y (VAR "x")` by SRW_TAC [][LAM_eq_thm] THEN
+  POP_ASSUM SUBST1_TAC THEN
+  ASM_SIMP_TAC (bsrw_ss()) [] THEN
+  `∀x y. (x = y) ⇒ (x == y)` by SRW_TAC [][] THEN POP_ASSUM MATCH_MP_TAC THEN
   SRW_TAC [boolSimps.CONJ_ss][LAM_eq_thm, tpm_fresh, NOT_IN_SUB]);
 
 val S_I = store_thm(
   "S_I",
-  ``v ∈ FV M ∧ v ∈ FV N ∧ N ≠ VAR v ⇒ 
+  ``v ∈ FV M ∧ v ∈ FV N ⇒
     LAM v (M @@ N) == S @@ (LAM v M) @@ (LAM v N)``,
-  STRIP_TAC THEN REWRITE_TAC [chap2Theory.S_def] THEN 
-  Q_TAC (NEW_TAC "z") `{"x"; "y"; "z"} ∪ FV M ∪ FV N` THEN 
-  `LAM "z" (VAR "x" @@ VAR "z" @@ (VAR "y" @@ VAR "z")) = 
+  STRIP_TAC THEN REWRITE_TAC [chap2Theory.S_def] THEN
+  Q_TAC (NEW_TAC "z") `{"x"; "y"; "z"} ∪ FV M ∪ FV N` THEN
+  `LAM "z" (VAR "x" @@ VAR "z" @@ (VAR "y" @@ VAR "z")) =
    LAM z (VAR "x" @@ VAR z @@ (VAR "y" @@ VAR z))`
-     by SRW_TAC [][LAM_eq_thm] THEN 
-  POP_ASSUM SUBST1_TAC THEN 
-  Q_TAC (NEW_TAC "y") `{"x"; "y"; z} ∪ FV M ∪ FV N` THEN 
+     by SRW_TAC [][LAM_eq_thm] THEN
+  POP_ASSUM SUBST1_TAC THEN
+  Q_TAC (NEW_TAC "y") `{"x"; "y"; z} ∪ FV M ∪ FV N` THEN
   `LAM "y" (LAM z (VAR "x" @@ VAR z @@ (VAR "y" @@ VAR z))) =
    LAM y (LAM z (VAR "x" @@ VAR z @@ (VAR y @@ VAR z)))`
-     by SRW_TAC [][LAM_eq_thm] THEN 
-  POP_ASSUM SUBST1_TAC THEN 
-  ASM_SIMP_TAC (bsrw_ss()) [NOT_IN_SUB] THEN 
+     by SRW_TAC [][LAM_eq_thm] THEN
+  POP_ASSUM SUBST1_TAC THEN
+  ASM_SIMP_TAC (bsrw_ss()) [NOT_IN_SUB] THEN
   `LAM v (M @@ N) = LAM z ([VAR z/v] (M @@ N))`
-     by SRW_TAC [][SIMPLE_ALPHA] THEN 
+     by SRW_TAC [][SIMPLE_ALPHA] THEN
   SRW_TAC [][]);
 
 val fake_eta = store_thm(
   "fake_eta",
   ``v ∉ FV M ∧ is_abs M ⇒ (LAM v (M @@ VAR v) == M)``,
-  STRIP_TAC THEN 
+  STRIP_TAC THEN
   `∃u M0. M = LAM u M0`
-     by (Q.SPEC_THEN `M` FULL_STRUCT_CASES_TAC term_CASES THEN 
-         FULL_SIMP_TAC (srw_ss()) [] THEN METIS_TAC []) THEN 
-  ASM_SIMP_TAC (bsrw_ss()) [] THEN 
-  FULL_SIMP_TAC (srw_ss()) [] THEN 
-  Cases_on `v = u` THEN SRW_TAC [][] THEN RES_TAC THEN 
-  `LAM u M0 = LAM v ([VAR v/u] M0)` by SRW_TAC [][SIMPLE_ALPHA] THEN 
+     by (Q.SPEC_THEN `M` FULL_STRUCT_CASES_TAC term_CASES THEN
+         FULL_SIMP_TAC (srw_ss()) [] THEN METIS_TAC []) THEN
+  ASM_SIMP_TAC (bsrw_ss()) [] THEN
+  FULL_SIMP_TAC (srw_ss()) [] THEN
+  Cases_on `v = u` THEN SRW_TAC [][] THEN RES_TAC THEN
+  `LAM u M0 = LAM v ([VAR v/u] M0)` by SRW_TAC [][SIMPLE_ALPHA] THEN
   SRW_TAC [][]);
 
 
 val B_eta = store_thm(
   "B_eta",
   ``LAM v (B @@ VAR v) == B``,
-  SIMP_TAC (bsrw_ss()) [chap2Theory.B_def] THEN 
+  SIMP_TAC (bsrw_ss()) [chap2Theory.B_def] THEN
   `S @@ (K @@ S) @@ K =
-   LAM "x" (LAM "y" (LAM "z" (VAR "x" @@ VAR "z" @@ (VAR "y" @@ VAR "z")))) @@ 
+   LAM "x" (LAM "y" (LAM "z" (VAR "x" @@ VAR "z" @@ (VAR "y" @@ VAR "z")))) @@
        (K @@ S) @@ K`
-     by SRW_TAC [][chap2Theory.S_def] THEN 
-  ASM_SIMP_TAC (bsrw_ss()) [] THEN 
-  `∀x y. (x = y) ⇒ x == y` by SRW_TAC [][] THEN 
-  POP_ASSUM MATCH_MP_TAC THEN 
+     by SRW_TAC [][chap2Theory.S_def] THEN
+  ASM_SIMP_TAC (bsrw_ss()) [] THEN
+  `∀x y. (x = y) ⇒ x == y` by SRW_TAC [][] THEN
+  POP_ASSUM MATCH_MP_TAC THEN
   SRW_TAC [][LAM_eq_thm, tpm_fresh]);
 
 val eqn_elim = prove(
   ``(∀Y. X:term == Y ⇔ Z == Y) ⇒ X == Z``,
   METIS_TAC [chap2Theory.lam_eq_rules]);
-fun brackabs_equiv ths def = let 
+fun brackabs_equiv ths def = let
   val lameq_t = ``chap2$==``
-  val th = if is_eq (concl def) then let 
+  val th = if is_eq (concl def) then let
                val (l,r) = dest_eq (concl def)
              in
                EQ_MP (AP_TERM (mk_comb(lameq_t, l)) def)
@@ -439,11 +439,11 @@ fun brackabs_equiv ths def = let
              end
            else def
 in
-  SIMP_RULE (bsrw_ss()) 
+  SIMP_RULE (bsrw_ss())
             ([S_I, K_I, B_I, C_I, fake_eta, B_eta, I_I] @ ths)
             th
 end
-  
+
 val is_abs_cdV = Store_thm(
   "is_abs_cdV",
   ``is_abs cdV``,
@@ -460,21 +460,21 @@ val termrec_var_def = Define`
 val termrec_var_eta = store_thm(
   "termrec_var_eta",
   ``LAM x (termrec_var @@ VAR x) == termrec_var``,
-  SIMP_TAC (bsrw_ss()) [termrec_var_def] THEN 
-  REWRITE_TAC [chap2Theory.S_def] THEN 
-  SIMP_TAC (bsrw_ss()) [] THEN 
-  `∀x y. (x = y) ⇒ x == y` by SRW_TAC [][] THEN 
-  POP_ASSUM MATCH_MP_TAC THEN 
-  SRW_TAC [boolSimps.CONJ_ss][LAM_eq_thm, tpm_fresh] THEN 
-  Cases_on `x = "z"` THEN SRW_TAC [][lemma14b] THEN 
+  SIMP_TAC (bsrw_ss()) [termrec_var_def] THEN
+  REWRITE_TAC [chap2Theory.S_def] THEN
+  SIMP_TAC (bsrw_ss()) [] THEN
+  `∀x y. (x = y) ⇒ x == y` by SRW_TAC [][] THEN
+  POP_ASSUM MATCH_MP_TAC THEN
+  SRW_TAC [boolSimps.CONJ_ss][LAM_eq_thm, tpm_fresh] THEN
+  Cases_on `x = "z"` THEN SRW_TAC [][lemma14b] THEN
   SRW_TAC [][GSYM fresh_tpm_subst, tpm_fresh]);
-  
+
 
 val termrec_comb_def = Define`
-  termrec_comb = 
-  LAM "c" (LAM "r1" (LAM "r2" 
+  termrec_comb =
+  LAM "c" (LAM "r1" (LAM "r2"
     (cpair @@ (cdAPP @@ (cfst @@ VAR "r1") @@ (cfst @@ VAR "r2"))
-           @@ (VAR "c" 
+           @@ (VAR "c"
                    @@ (cfst @@ VAR "r1") @@ (cfst @@ VAR "r2")
                    @@ (csnd @@ VAR "r1") @@ (csnd @@ VAR "r2")))))
 `;
@@ -482,8 +482,8 @@ val termrec_comb_eqn = brackabs_equiv [] termrec_comb_def
 
 
 val termrec_abs_def = Define`
-  termrec_abs = 
-  LAM "a" (LAM "r" 
+  termrec_abs =
+  LAM "a" (LAM "r"
     (cpair @@ (cdABS @@ (cfst @@ VAR "r"))
            @@ (VAR "a" @@ (cfst @@ VAR "r") @@ (csnd @@ VAR "r"))))
 `;
@@ -501,21 +501,21 @@ val is_abs_termrecsubs = Store_thm(
 
 val fst_termrec_subs = store_thm(
   "fst_termrec_subs",
-  ``∀t. cfst @@ (cDB t 
-                     @@ (termrec_var @@ v) 
+  ``∀t. cfst @@ (cDB t
+                     @@ (termrec_var @@ v)
                      @@ (termrec_comb @@ c)
-                     @@ (termrec_abs @@ a)) == 
+                     @@ (termrec_abs @@ a)) ==
         cDB t``,
   SIMP_TAC (bsrw_ss()) [termrec_var_def, termrec_comb_eqn, termrec_abs_eqn] THEN
-  Induct THEN ASM_SIMP_TAC (bsrw_ss()) [cDB_thm, 
-                                        churchpairTheory.cfst_pair, 
-                                        cdV_behaviour, cdAPP_behaviour, 
+  Induct THEN ASM_SIMP_TAC (bsrw_ss()) [cDB_thm,
+                                        churchpairTheory.cfst_pair,
+                                        cdV_behaviour, cdAPP_behaviour,
                                         cdABS_behaviour]);
 
 val termrec_def = Define`
-  termrec = 
+  termrec =
   LAM "v" (LAM "c" (LAM "a" (LAM "t"
-    (csnd @@ (VAR "t" 
+    (csnd @@ (VAR "t"
                   @@ (termrec_var @@ VAR "v")
                   @@ (termrec_comb @@ VAR "c")
                   @@ (termrec_abs @@ VAR "a"))))))
@@ -534,38 +534,38 @@ val termrec_behaviour = store_thm(
   "termrec_behaviour",
   ``termrec @@ v @@ c @@ a @@ cDB (dV i) == v @@ church i ∧
     termrec @@ v @@ c @@ a @@ cDB (dAPP t u) ==
-      c @@ cDB t @@ cDB u 
+      c @@ cDB t @@ cDB u
         @@ (termrec @@ v @@ c @@ a @@ cDB t)
         @@ (termrec @@ v @@ c @@ a @@ cDB u) ∧
     termrec @@ v @@ c @@ a @@ cDB (dABS t) ==
       a @@ cDB t @@ (termrec @@ v @@ c @@ a @@ cDB t)``,
   REPEAT CONJ_TAC THENL [
-    SIMP_TAC (bsrw_ss()) [termrec_eqn, cDB_thm, termrec_var_def, 
+    SIMP_TAC (bsrw_ss()) [termrec_eqn, cDB_thm, termrec_var_def,
                           churchpairTheory.csnd_pair],
 
-    SIMP_TAC (bsrw_ss()) [termrec_eqn, cDB_thm] THEN 
-    ASSUME_TAC (``termrec_comb @@ c @@ x @@ y == X`` 
+    SIMP_TAC (bsrw_ss()) [termrec_eqn, cDB_thm] THEN
+    ASSUME_TAC (``termrec_comb @@ c @@ x @@ y == X``
                   |> SIMP_CONV (bsrw_ss()) [termrec_comb_eqn]
                   |> Q.GEN `X`
-                  |> MATCH_MP eqn_elim 
-                  |> Q.GEN `y` |> Q.GEN `x`) THEN 
+                  |> MATCH_MP eqn_elim
+                  |> Q.GEN `y` |> Q.GEN `x`) THEN
     ASM_SIMP_TAC (bsrw_ss()) [churchpairTheory.csnd_pair, fst_termrec_subs],
-    
-    SIMP_TAC (bsrw_ss()) [termrec_eqn, cDB_thm] THEN 
-    ASSUME_TAC (``termrec_abs @@ a @@ x == X`` 
+
+    SIMP_TAC (bsrw_ss()) [termrec_eqn, cDB_thm] THEN
+    ASSUME_TAC (``termrec_abs @@ a @@ x == X``
                   |> SIMP_CONV (bsrw_ss()) [termrec_abs_eqn]
                   |> Q.GEN `X`
-                  |> MATCH_MP eqn_elim 
-                  |> Q.GEN `x`) THEN 
+                  |> MATCH_MP eqn_elim
+                  |> Q.GEN `x`) THEN
     ASM_SIMP_TAC (bsrw_ss()) [churchpairTheory.csnd_pair, fst_termrec_subs]
   ]);
 
-(* ---------------------------------------------------------------------- 
+(* ----------------------------------------------------------------------
     cis_abs - is a term an abstraction?
    ---------------------------------------------------------------------- *)
 
 val cis_abs_def = Define`
-  cis_abs = 
+  cis_abs =
   LAM "t" (VAR "t" @@ (K @@ cB F) @@ (K @@ (K @@ cB F)) @@ (K @@ cB T))
 `;
 
@@ -586,15 +586,15 @@ val is_abs_cis_abs = Store_thm(
 val cis_abs_behaviour = store_thm(
   "cis_abs_behaviour",
   ``cis_abs @@ cDB t -n->* cB (is_dABS t)``,
-  SIMP_TAC (bsrw_ss()) [cis_abs_def] THEN Cases_on `t` THEN 
-  SIMP_TAC (bsrw_ss()) [cDB_thm]); 
+  SIMP_TAC (bsrw_ss()) [cis_abs_def] THEN Cases_on `t` THEN
+  SIMP_TAC (bsrw_ss()) [cDB_thm]);
 
 (* ----------------------------------------------------------------------
     cbnf - is a term in β-nf?
    ---------------------------------------------------------------------- *)
 
 val cbnf_def = Define`
-  cbnf = 
+  cbnf =
   termrec @@ (LAM "i" (cB T))
           @@ (LAM "t1" (LAM "t2" (LAM "r1" (LAM "r2"
                 (cand @@ VAR "r1"
@@ -606,20 +606,20 @@ val cbnf_def = Define`
 val FV_cbnf = Store_thm(
   "FV_cbnf",
   ``FV cbnf = {}``,
-  SRW_TAC [][cbnf_def, EXTENSION]); 
+  SRW_TAC [][cbnf_def, EXTENSION]);
 
 
 val cbnf_equiv = brackabs_equiv [] cbnf_def
 val cbnf_behaviour = store_thm(
   "cbnf_behaviour",
   ``cbnf @@ cDB t -n->* cB (dbnf t)``,
-  SIMP_TAC (bsrw_ss()) [cbnf_equiv] THEN 
-  Induct_on `t` THEN 
-  ASM_SIMP_TAC (bsrw_ss()) [termrec_behaviour, cand_behaviour, 
+  SIMP_TAC (bsrw_ss()) [cbnf_equiv] THEN
+  Induct_on `t` THEN
+  ASM_SIMP_TAC (bsrw_ss()) [termrec_behaviour, cand_behaviour,
                             cis_abs_behaviour, cnot_behaviour]);
 
-(* ---------------------------------------------------------------------- 
-    cnsub - the computable version of nsub, which has defining equations 
+(* ----------------------------------------------------------------------
+    cnsub - the computable version of nsub, which has defining equations
        (nsub s k (dV i) = if k < i then dV (i - 1)
                           else if i = k then s else dV i) /\
        (nsub s k (dAPP t u) = dAPP (nsub s k t) (nsub s k u)) /\
@@ -627,20 +627,20 @@ val cbnf_behaviour = store_thm(
    ---------------------------------------------------------------------- *)
 
 val cnsub_def = Define`
-  cnsub = 
-  LAM "s" (LAM "k" (LAM "t" 
-   (VAR "t" 
+  cnsub =
+  LAM "s" (LAM "k" (LAM "t"
+   (VAR "t"
         @@ (LAM "i" (LAM "s" (LAM "k"
               (cless @@ VAR "k" @@ VAR "i"  (* if k < i *)
                      @@ (cdV @@ (cminus @@ VAR "i" @@ church 1)) (* then *)
                      @@ (ceqnat @@ VAR "i" @@ VAR "k" (* if i = k *)
-                                @@ VAR "s" 
+                                @@ VAR "s"
                                 @@ (cdV @@ VAR "i"))))))
         @@ (LAM "r1" (LAM "r2" (LAM "s" (LAM "k"
               (cdAPP @@ (VAR "r1" @@ VAR "s" @@ VAR "k")
                      @@ (VAR "r2" @@ VAR "s" @@ VAR "k"))))))
         @@ (LAM "r" (LAM "s" (LAM "k"
-              (cdABS @@ (VAR "r" 
+              (cdABS @@ (VAR "r"
                              @@ (clift @@ VAR "s" @@ church 0)
                              @@ (cplus @@ VAR "k" @@ church 1))))))
         @@ VAR "s" @@ VAR "k")))
@@ -657,12 +657,12 @@ val is_abs_cnsub = Store_thm(
 
 val Ccless_eta = prove(
   ``LAM x (C @@ cless @@ VAR x) == C @@ cless``,
-  SIMP_TAC (bsrw_ss()) [chap2Theory.C_def] THEN 
-  SIMP_TAC (bsrw_ss()) [chap2Theory.B_def] THEN 
-  CONV_TAC (RAND_CONV (SIMP_CONV (bsrw_ss()) [Once chap2Theory.S_def])) THEN 
-  SIMP_TAC (bsrw_ss()) [] THEN 
-  `∀x y. (x = y) ⇒ (x == y)` by SRW_TAC [][] THEN 
-  POP_ASSUM MATCH_MP_TAC THEN 
+  SIMP_TAC (bsrw_ss()) [chap2Theory.C_def] THEN
+  SIMP_TAC (bsrw_ss()) [chap2Theory.B_def] THEN
+  CONV_TAC (RAND_CONV (SIMP_CONV (bsrw_ss()) [Once chap2Theory.S_def])) THEN
+  SIMP_TAC (bsrw_ss()) [] THEN
+  `∀x y. (x = y) ⇒ (x == y)` by SRW_TAC [][] THEN
+  POP_ASSUM MATCH_MP_TAC THEN
   SRW_TAC [][LAM_eq_thm, tpm_fresh]);
 
 val cnsub_equiv0 = brackabs_equiv [Ccless_eta] cnsub_def
@@ -671,16 +671,16 @@ val cnsub_equiv = brackabs_equiv [B_I_uncond] cnsub_equiv0
 val cnsub_behaviour = store_thm(
   "cnsub_behaviour",
   ``∀u i t. cnsub @@ cDB t @@ church i @@ cDB u -n->* cDB (nsub t i u)``,
-  SIMP_TAC (bsrw_ss()) [cnsub_equiv] THEN 
+  SIMP_TAC (bsrw_ss()) [cnsub_equiv] THEN
   Induct THEN
-  ASM_SIMP_TAC (bsrw_ss()) [cDB_thm, cminus_behaviour, cdV_behaviour, 
-                            cless_behaviour, ceqnat_behaviour, 
-                            cdAPP_behaviour, clift_behaviour, 
-                            cplus_behaviour, cdABS_behaviour] THEN 
+  ASM_SIMP_TAC (bsrw_ss()) [cDB_thm, cminus_behaviour, cdV_behaviour,
+                            cless_behaviour, ceqnat_behaviour,
+                            cdAPP_behaviour, clift_behaviour,
+                            cplus_behaviour, cdABS_behaviour] THEN
   SRW_TAC [][] THEN ASM_SIMP_TAC (bsrw_ss()) [cB_behaviour]);
 
-(* ---------------------------------------------------------------------- 
-    norm_reduct - get the normal order reduct, if there is one. 
+(* ----------------------------------------------------------------------
+    norm_reduct - get the normal order reduct, if there is one.
                   If there isn't, just return something unspecified.
 
       (noreduct (LAM v M) = OPTION_MAP (LAM v) (noreduct M)) ∧
@@ -689,18 +689,18 @@ val cnsub_behaviour = store_thm(
                     if bnf M then OPTION_MAP ((@@) M) (noreduct N)
                     else OPTION_MAP (λM'. M' @@ N) (noreduct M))) ∧
       (noreduct (VAR s) = NONE)
-    
+
     We can ignore all the option_map cruft.
    ---------------------------------------------------------------------- *)
 
 val cnoreduct_def = Define`
-  cnoreduct = 
-  termrec 
+  cnoreduct =
+  termrec
     @@ (LAM "i" (cdV @@ VAR "i"))
     @@ (LAM "t0" (LAM "t1" (LAM "r0" (LAM "r1"
           (cis_abs @@ VAR "t0"  (* if left term is abstraction *)
-                   @@ (cnsub @@ VAR "t1" 
-                             @@ church 0 
+                   @@ (cnsub @@ VAR "t1"
+                             @@ church 0
                              @@ (termrec @@ I @@ I @@ K @@ VAR "t0"))
                    @@ (cbnf @@ VAR "t0" (* if left term is in bnf *)
                             @@ (cdAPP @@ VAR "t0" @@ VAR "r1")
@@ -719,102 +719,102 @@ val cnoreduct_equiv = brackabs_equiv [B_I_uncond] cnoreduct_equiv0
 val cnoreduct_behaviour = store_thm(
   "cnoreduct_behaviour",
   ``∀t. ¬bnf t ⇒
-           cnoreduct @@ cDB (fromTerm t) -n->* 
+           cnoreduct @@ cDB (fromTerm t) -n->*
            cDB (fromTerm (THE (noreduct t)))``,
-  SIMP_TAC (bsrw_ss()) [cnoreduct_equiv] THEN 
-  Q.MATCH_ABBREV_TAC 
+  SIMP_TAC (bsrw_ss()) [cnoreduct_equiv] THEN
+  Q.MATCH_ABBREV_TAC
     `∀t. ¬bnf t ⇒ termrec @@ cdV @@ COMB @@ ABS @@ cDB (fromTerm t) ==
-                   cDB (fromTerm (THE (noreduct t)))` THEN 
-  completeInduct_on `size t` THEN Q.X_GEN_TAC `t` THEN 
-  FULL_SIMP_TAC (srw_ss() ++ boolSimps.DNF_ss) [] THEN 
+                   cDB (fromTerm (THE (noreduct t)))` THEN
+  completeInduct_on `size t` THEN Q.X_GEN_TAC `t` THEN
+  FULL_SIMP_TAC (srw_ss() ++ boolSimps.DNF_ss) [] THEN
   Q.SPEC_THEN `t` FULL_STRUCT_CASES_TAC term_CASES THENL [
     SRW_TAC [][],
     Cases_on `is_abs t1` THENL [
-      ASM_SIMP_TAC (bsrw_ss()) [termrec_behaviour, Abbr`COMB`, 
-                                cis_abs_behaviour, cB_behaviour] THEN 
+      ASM_SIMP_TAC (bsrw_ss()) [termrec_behaviour, Abbr`COMB`,
+                                cis_abs_behaviour, cB_behaviour] THEN
       `∃v t0. t1 = LAM v t0`
          by (Q.SPEC_THEN `t1` FULL_STRUCT_CASES_TAC term_CASES THEN
-             FULL_SIMP_TAC (srw_ss()) [] THEN METIS_TAC[]) THEN 
-      ASM_SIMP_TAC (bsrw_ss()) [dLAM_def, termrec_behaviour, 
-                                cnsub_behaviour, GSYM sub_nsub, 
-                                noreduct_thm, 
+             FULL_SIMP_TAC (srw_ss()) [] THEN METIS_TAC[]) THEN
+      ASM_SIMP_TAC (bsrw_ss()) [dLAM_def, termrec_behaviour,
+                                cnsub_behaviour, GSYM sub_nsub,
+                                noreduct_thm,
                                 GSYM fromTerm_subst],
 
       Cases_on `bnf t1` THEN
-      ASM_SIMP_TAC (bsrw_ss() ++ ARITH_ss) 
-                   [termrec_behaviour, Abbr`COMB`, 
-                    cis_abs_behaviour, cB_behaviour, 
-                    cbnf_behaviour, cdAPP_behaviour, 
-                    noreduct_thm] 
+      ASM_SIMP_TAC (bsrw_ss() ++ ARITH_ss)
+                   [termrec_behaviour, Abbr`COMB`,
+                    cis_abs_behaviour, cB_behaviour,
+                    cbnf_behaviour, cdAPP_behaviour,
+                    noreduct_thm]
       THENL [
-        Cases_on `noreduct t2` THEN 
+        Cases_on `noreduct t2` THEN
         FULL_SIMP_TAC (srw_ss()) [noreduct_bnf],
-        Cases_on `noreduct t1` THEN 
+        Cases_on `noreduct t1` THEN
         FULL_SIMP_TAC (srw_ss()) [noreduct_bnf]
       ]
     ],
 
-    ASM_SIMP_TAC (bsrw_ss()) [Abbr`ABS`, termrec_behaviour, dLAM_def] THEN 
-    Q.RM_ABBREV_TAC `COMB` THEN 
-    Q.MATCH_ABBREV_TAC `(v = size t0 + 1) ⇒ 
-                        ¬bnf t0 ⇒ 
-                        cdABS @@ (termrec @@ cdV @@ COMB @@ (K @@ cdABS) 
+    ASM_SIMP_TAC (bsrw_ss()) [Abbr`ABS`, termrec_behaviour, dLAM_def] THEN
+    Q.RM_ABBREV_TAC `COMB` THEN
+    Q.MATCH_ABBREV_TAC `(v = size t0 + 1) ⇒
+                        ¬bnf t0 ⇒
+                        cdABS @@ (termrec @@ cdV @@ COMB @@ (K @@ cdABS)
                                           @@ cDB XX) ==
-                        cDB (fromTerm (THE (noreduct (LAM u t0))))` THEN 
-    Q.ABBREV_TAC 
+                        cDB (fromTerm (THE (noreduct (LAM u t0))))` THEN
+    Q.ABBREV_TAC
       `YY = [VAR (n2s 0)/n2s (s2n u + 1)] (toTerm (lift (fromTerm t0) 0))` THEN
-    `XX = fromTerm YY` by SRW_TAC [][fromTerm_subst, Abbr`XX`, Abbr`YY`] THEN 
-    REPEAT STRIP_TAC THEN 
-    Q.ABBREV_TAC `MX = if dFV (fromTerm t0) = {} then 0 
-                       else MAX_SET (dFV (fromTerm t0))` THEN 
+    `XX = fromTerm YY` by SRW_TAC [][fromTerm_subst, Abbr`XX`, Abbr`YY`] THEN
+    REPEAT STRIP_TAC THEN
+    Q.ABBREV_TAC `MX = if dFV (fromTerm t0) = {} then 0
+                       else MAX_SET (dFV (fromTerm t0))` THEN
     `∀i. i ∈ dFV (fromTerm t0) ⇒ i ≤ MX`
-       by SRW_TAC [][Abbr`MX`, MAX_SET_DEF] THEN 
-    Q.ABBREV_TAC `π = lifting_pm 0 MX` THEN 
+       by SRW_TAC [][Abbr`MX`, MAX_SET_DEF] THEN
+    Q.ABBREV_TAC `π = lifting_pm 0 MX` THEN
     `lift (fromTerm t0) 0 = dpm π (fromTerm t0)`
-       by SRW_TAC [][lifts_are_specific_dpms, Abbr`π`] THEN 
-    `_ = fromTerm (tpm π t0)` by METIS_TAC [fromTerm_swap_invariant] THEN 
+       by SRW_TAC [][lifts_are_specific_dpms, Abbr`π`] THEN
+    `_ = fromTerm (tpm π t0)` by METIS_TAC [fromTerm_swap_invariant] THEN
     `YY = [VAR (n2s 0)/n2s (s2n u + 1)] (tpm π t0)`
-        by METIS_TAC [tofromTerm] THEN 
-    `size YY = size t0` by SRW_TAC [][] THEN 
-    `¬bnf YY` by SRW_TAC [][] THEN 
-    `size YY < v` by DECIDE_TAC THEN 
-    Q.PAT_ASSUM `YY = ZZZ` (ASSUME_TAC o SYM) THEN 
-    ASM_SIMP_TAC (bsrw_ss()) [cdABS_behaviour, 
-                              noreduct_thm] THEN 
+        by METIS_TAC [tofromTerm] THEN
+    `size YY = size t0` by SRW_TAC [][] THEN
+    `¬bnf YY` by SRW_TAC [][] THEN
+    `size YY < v` by DECIDE_TAC THEN
+    Q.PAT_ASSUM `YY = ZZZ` (ASSUME_TAC o SYM) THEN
+    ASM_SIMP_TAC (bsrw_ss()) [cdABS_behaviour,
+                              noreduct_thm] THEN
     `(noreduct t0 = NONE) ∨ (∃tt. noreduct t0 = SOME tt)`
        by (Cases_on `noreduct t0` THEN SRW_TAC [][]) THEN1
-      FULL_SIMP_TAC (srw_ss()) [noreduct_bnf] THEN 
-    ASM_SIMP_TAC (srw_ss()) [dLAM_def] THEN 
-    SRW_TAC [][noreduct_vsubst, noreduct_tpm, fromTerm_subst] THEN 
-    REWRITE_TAC [GSYM fromTerm_swap_invariant] THEN 
+      FULL_SIMP_TAC (srw_ss()) [noreduct_bnf] THEN
+    ASM_SIMP_TAC (srw_ss()) [dLAM_def] THEN
+    SRW_TAC [][noreduct_vsubst, noreduct_tpm, fromTerm_subst] THEN
+    REWRITE_TAC [GSYM fromTerm_swap_invariant] THEN
     `∀i. i ∈ dFV (fromTerm tt) ⇒ i ∈ dFV (fromTerm t0)`
-       by (`t0 -n-> tt` by METIS_TAC [noreduct_characterisation] THEN 
-           `t0 -β-> tt` by IMP_RES_TAC normorder_ccbeta THEN 
-           `FV tt ⊆ FV t0` by IMP_RES_TAC chap3Theory.cc_beta_FV_SUBSET THEN 
-           `∀v. v ∈ FV tt ⇒ v ∈ FV t0` by METIS_TAC [SUBSET_DEF] THEN 
+       by (`t0 -n-> tt` by METIS_TAC [noreduct_characterisation] THEN
+           `t0 -β-> tt` by IMP_RES_TAC normorder_ccbeta THEN
+           `FV tt ⊆ FV t0` by IMP_RES_TAC chap3Theory.cc_beta_FV_SUBSET THEN
+           `∀v. v ∈ FV tt ⇒ v ∈ FV t0` by METIS_TAC [SUBSET_DEF] THEN
            `∀v. v ∈ dFVs (fromTerm tt) ⇒ v ∈ dFVs (fromTerm t0)`
-              by SRW_TAC [][dFVs_fromTerm] THEN 
-           SRW_TAC [][IN_dFV]) THEN 
-    `∀i. i ∈ dFV (fromTerm tt) ⇒ i ≤ MX` by METIS_TAC [] THEN 
+              by SRW_TAC [][dFVs_fromTerm] THEN
+           SRW_TAC [][IN_dFV]) THEN
+    `∀i. i ∈ dFV (fromTerm tt) ⇒ i ≤ MX` by METIS_TAC [] THEN
     `lift (fromTerm tt) 0 = dpm π (fromTerm tt)`
-      by SRW_TAC [][lifts_are_specific_dpms, Abbr`π`] THEN 
+      by SRW_TAC [][lifts_are_specific_dpms, Abbr`π`] THEN
     SRW_TAC [][fromTerm_swap_invariant]
   ]);
-      
-val cnoreduct_behaviour' = 
+
+val cnoreduct_behaviour' =
     SIMP_RULE (srw_ss()) [] (SPEC ``toTerm d`` cnoreduct_behaviour)
-  
-(* ---------------------------------------------------------------------- 
-    cichurch 
+
+(* ----------------------------------------------------------------------
+    cichurch
 
     create the internal structure of a church numeral (what is done by
     FUNPOW in the HOL world)
    ---------------------------------------------------------------------- *)
 
 val cichurch_def = Define`
-  cichurch = 
-  LAM "n" 
-    (VAR "n" 
+  cichurch =
+  LAM "n"
+    (VAR "n"
        @@ (cdV @@ church 1)
        @@ (LAM "r" (cdAPP @@ (cdV @@ church 0) @@ VAR "r")))
 `;
@@ -830,7 +830,7 @@ val cichurch_behaviour = store_thm(
   "cichurch_behaviour",
   ``cichurch @@ church n -n->* cDB (fromTerm (FUNPOW ((@@) (VAR (n2s 0))) n
                                                      (VAR (n2s 1))))``,
-  SIMP_TAC (bsrw_ss()) [cichurch_def, cdV_behaviour] THEN 
+  SIMP_TAC (bsrw_ss()) [cichurch_def, cdV_behaviour] THEN
   Induct_on `n` THEN
   ASM_SIMP_TAC (bsrw_ss()) [church_thm, cdV_behaviour, cdAPP_behaviour,
                             FUNPOW_SUC]);
@@ -839,7 +839,7 @@ val cichurch_behaviour = store_thm(
     cchurch
 
     Puts the abstractions over the internal church structure, giving an
-    encoded church numeral 
+    encoded church numeral
    ---------------------------------------------------------------------- *)
 
 val cchurch_def = Define`
@@ -853,7 +853,7 @@ val FV_cchurch = Store_thm(
 
 val fromTerm_funpow_app = store_thm(
   "fromTerm_funpow_app",
-  ``fromTerm (FUNPOW ((@@) f) n x) = 
+  ``fromTerm (FUNPOW ((@@) f) n x) =
       FUNPOW (dAPP (fromTerm f)) n (fromTerm x)``,
   Induct_on `n` THEN SRW_TAC [][FUNPOW_SUC]);
 
@@ -870,27 +870,27 @@ val sub_funpow_dAPP = store_thm(
 val cchurch_behaviour = store_thm(
   "cchurch_behaviour",
   ``cchurch @@ church n -n->* cDB (fromTerm (church n))``,
-  SIMP_TAC (bsrw_ss()) [cchurch_def, cichurch_behaviour] THEN 
-  SIMP_TAC (bsrw_ss()) [church_def, cdABS_behaviour, fromTerm_funpow_app, 
-                        dLAM_def, lift_funpow_dAPP, sub_funpow_dAPP] THEN 
+  SIMP_TAC (bsrw_ss()) [cchurch_def, cichurch_behaviour] THEN
+  SIMP_TAC (bsrw_ss()) [church_def, cdABS_behaviour, fromTerm_funpow_app,
+                        dLAM_def, lift_funpow_dAPP, sub_funpow_dAPP] THEN
   SIMP_TAC (srw_ss() ++ ARITH_ss) []);
 
 val _ = temp_overload_on ("LAMvca", ``λM. LAM "v" (LAM "c" (LAM "a" M))``)
 
 (* ----------------------------------------------------------------------
-    cciDB : the encoded/computing version of ciDB 
+    cciDB : the encoded/computing version of ciDB
    ---------------------------------------------------------------------- *)
 
 val cciDB_def = Define`
-  cciDB = LAM "t" 
-           (VAR "t" 
-             @@ (LAM "i" 
+  cciDB = LAM "t"
+           (VAR "t"
+             @@ (LAM "i"
                   (cdAPP @@ (cdV @@ church (s2n "v")) @@ (cchurch @@ VAR "i")))
              @@ (LAM "r1" (LAM "r2"
-                    (cdAPP 
+                    (cdAPP
                        @@ (cdAPP @@ (cdV @@ church (s2n "c")) @@ VAR "r1")
                        @@ VAR "r2")))
-             @@ (LAM "r" 
+             @@ (LAM "r"
                     (cdAPP @@ (cdV @@ church (s2n "a")) @@ VAR "r")))
 `;
 
@@ -902,19 +902,19 @@ val FV_cciDB = Store_thm(
 val cciDB_behaviour = store_thm(
   "cciDB_behaviour",
   ``cciDB @@ cDB dBt -n->* cDB (fromTerm (ciDB dBt))``,
-  SIMP_TAC (bsrw_ss()) [cciDB_def, cdV_behaviour] THEN 
+  SIMP_TAC (bsrw_ss()) [cciDB_def, cdV_behaviour] THEN
   Induct_on `dBt` THEN
-  ASM_SIMP_TAC (bsrw_ss()) [cDB_thm, cdV_behaviour, cchurch_behaviour, 
-                            cdAPP_behaviour] THEN 
+  ASM_SIMP_TAC (bsrw_ss()) [cDB_thm, cdV_behaviour, cchurch_behaviour,
+                            cdAPP_behaviour] THEN
   ASM_SIMP_TAC (bsrw_ss()) [ciDB_def]);
 
 (* ----------------------------------------------------------------------
-    ccDB : the encoded version of cDB 
+    ccDB : the encoded version of cDB
    ---------------------------------------------------------------------- *)
 
 val ccDB_def = Define`
-  ccDB = LAM "t" (cdLAM @@ church (s2n "v") @@ 
-                    (cdLAM @@ church (s2n "c") @@ 
+  ccDB = LAM "t" (cdLAM @@ church (s2n "v") @@
+                    (cdLAM @@ church (s2n "c") @@
                        (cdLAM @@ church (s2n "a") @@ (cciDB @@ VAR "t"))))
 `;
 val FV_ccDB = Store_thm(
@@ -925,12 +925,12 @@ val FV_ccDB = Store_thm(
 val ccDB_behaviour = store_thm(
   "ccDB_behaviour",
   ``ccDB @@ (cDB dbt) -n->* cDB (fromTerm (cDB dbt))``,
-  SIMP_TAC (bsrw_ss()) [ccDB_def, cciDB_behaviour, cdLAM_behaviour] THEN 
-  Q.SPEC_THEN `dbt` ASSUME_TAC cDB_def THEN 
+  SIMP_TAC (bsrw_ss()) [ccDB_def, cciDB_behaviour, cdLAM_behaviour] THEN
+  Q.SPEC_THEN `dbt` ASSUME_TAC cDB_def THEN
   SRW_TAC [][]);
 
-(* ---------------------------------------------------------------------- 
-    enumerations are computable 
+(* ----------------------------------------------------------------------
+    enumerations are computable
    ---------------------------------------------------------------------- *)
 
 open enumerationsTheory
@@ -939,13 +939,13 @@ open enumerationsTheory
 
 
 val cdBnum_def = Define`
-  cdBnum = 
-  LAM "t" 
-    (VAR "t" 
+  cdBnum =
+  LAM "t"
+    (VAR "t"
          @@ (cmult @@ church 3)
-         @@ (LAM "r1" 
-               (B @@ csuc 
-                  @@ (B @@ (cmult @@ church 3) 
+         @@ (LAM "r1"
+               (B @@ csuc
+                  @@ (B @@ (cmult @@ church 3)
                         @@ (cnpair @@ VAR "r1"))))
          @@ (B @@ (cplus @@ church 2) @@ (cmult @@ church 3)))
 `;
@@ -958,14 +958,14 @@ val FV_cdBnum = Store_thm(
 val cdBnum_behaviour = store_thm(
   "cdBnum_behaviour",
   ``cdBnum @@ cDB t -n->* church (dBnum t)``,
-  SIMP_TAC (bsrw_ss()) [cdBnum_def] THEN Induct_on `t` THEN 
-  ASM_SIMP_TAC (bsrw_ss() ++ ARITH_ss) 
-               [cDB_thm, dBnum_def, cmult_behaviour, 
-                cnpair_behaviour, csuc_behaviour, 
+  SIMP_TAC (bsrw_ss()) [cdBnum_def] THEN Induct_on `t` THEN
+  ASM_SIMP_TAC (bsrw_ss() ++ ARITH_ss)
+               [cDB_thm, dBnum_def, cmult_behaviour,
+                cnpair_behaviour, csuc_behaviour,
                 arithmeticTheory.ADD1, cplus_behaviour]);
 
 val cndbsuc_def = Define`
-  cndbsuc = 
+  cndbsuc =
   LAM "r" (LAM "n" (LAM "m3" (LAM "d3"
              (cis_zero @@ VAR "m3"
               @@ (cdV @@ VAR "d3")
@@ -983,10 +983,10 @@ val FV_cndbsuc = Store_thm(
 
 val cndbsuc_dV_behaviour = store_thm(
   "cndbsuc_dV_behaviour",
-  ``(n MOD 3 = 0) ⇒ 
+  ``(n MOD 3 = 0) ⇒
     cndbsuc @@ r @@ church n -n->* cDB (dV (n DIV 3))``,
-  SIMP_TAC (bsrw_ss()) [cndbsuc_def] THEN FRESH_TAC THEN 
-  ASM_SIMP_TAC (bsrw_ss()) [tpm_fresh, cmod_behaviour, cis_zero_behaviour, 
+  SIMP_TAC (bsrw_ss()) [cndbsuc_def] THEN FRESH_TAC THEN
+  ASM_SIMP_TAC (bsrw_ss()) [tpm_fresh, cmod_behaviour, cis_zero_behaviour,
                             cB_behaviour, cdiv_behaviour, cdV_behaviour]);
 
 
@@ -999,32 +999,32 @@ val cndbsuc_eqn = brackabs_equiv [] cndbsuc_def
 
 val cndbsuc_dAPP_behaviour = store_thm(
   "cndbsuc_dAPP_behaviour",
-  ``(n MOD 3 ≠ 0) ∧ (n MOD 3 = 1) ⇒ 
-    cndbsuc @@ r @@ church n == 
-    cdAPP @@ (r @@ (cnfst @@ church (n DIV 3))) 
+  ``(n MOD 3 ≠ 0) ∧ (n MOD 3 = 1) ⇒
+    cndbsuc @@ r @@ church n ==
+    cdAPP @@ (r @@ (cnfst @@ church (n DIV 3)))
           @@ (r @@ (cnsnd @@ church (n DIV 3)))``,
-  STRIP_TAC THEN 
-  ASM_SIMP_TAC (bsrw_ss()) [cndbsuc_eqn, cmod_behaviour, cis_zero_behaviour, 
+  STRIP_TAC THEN
+  ASM_SIMP_TAC (bsrw_ss()) [cndbsuc_eqn, cmod_behaviour, cis_zero_behaviour,
                             ceqnat_behaviour, cB_behaviour, cdiv_behaviour]);
 
 val cndbsuc_dABS_behaviour = store_thm(
   "cndbsuc_dABS_behaviour",
   ``(n MOD 3 ≠ 0) ∧ (n MOD 3 ≠ 1) ⇒
     cndbsuc @@ r @@ church n == cdABS @@ (r @@ church (n DIV 3))``,
-  STRIP_TAC THEN 
-  ASM_SIMP_TAC (bsrw_ss()) [cndbsuc_eqn, cmod_behaviour, cis_zero_behaviour, 
+  STRIP_TAC THEN
+  ASM_SIMP_TAC (bsrw_ss()) [cndbsuc_eqn, cmod_behaviour, cis_zero_behaviour,
                             ceqnat_behaviour, cB_behaviour, cdiv_behaviour]);
- 
+
 val cnumdB0_def = Define`
-  cnumdB0 = 
-  natrec 
+  cnumdB0 =
+  natrec
    @@ (LAM "n" (cDB (dV 0)))
    @@ (LAM "c0" (LAM "r" (LAM "n"
        (ceqnat @@ (csuc @@ VAR "c0") @@ (VAR "n")
         @@ (cndbsuc @@ VAR "r" @@ VAR "n")
         @@ (VAR "r" @@ VAR "n")))))
 `;
-        
+
 val FV_cnumdB0 = Store_thm(
   "FV_cnumdB0",
   ``FV cnumdB0 = {}``,
@@ -1033,48 +1033,48 @@ val FV_cnumdB0 = Store_thm(
 val cnumdB0_behaviour = store_thm(
   "cnumdB0_behaviour",
   ``n ≤ c ⇒ cnumdB0 @@ church c @@ church n -n->* cDB (numdB n)``,
-  Q.ID_SPEC_TAC `n` THEN SIMP_TAC (bsrw_ss()) [cnumdB0_def] THEN 
+  Q.ID_SPEC_TAC `n` THEN SIMP_TAC (bsrw_ss()) [cnumdB0_def] THEN
   Induct_on `c` THEN
-  SIMP_TAC (bsrw_ss()) [natrec_behaviour, cdV_behaviour, 
-                        csuc_behaviour, cmod_behaviour, cdiv_behaviour, 
-                        ceqnat_behaviour] 
-  THEN1 SRW_TAC [][Once numdB_def] THEN 
-  REPEAT STRIP_TAC THEN Q.ABBREV_TAC `N = SUC c` THEN 
+  SIMP_TAC (bsrw_ss()) [natrec_behaviour, cdV_behaviour,
+                        csuc_behaviour, cmod_behaviour, cdiv_behaviour,
+                        ceqnat_behaviour]
+  THEN1 SRW_TAC [][Once numdB_def] THEN
+  REPEAT STRIP_TAC THEN Q.ABBREV_TAC `N = SUC c` THEN
   Cases_on `n = N` THENL [
-    SRW_TAC [][] THEN 
-    ASM_SIMP_TAC (bsrw_ss()) [cB_behaviour] THEN 
+    SRW_TAC [][] THEN
+    ASM_SIMP_TAC (bsrw_ss()) [cB_behaviour] THEN
     Cases_on `N MOD 3 = 0` THENL [
-      ASM_SIMP_TAC (bsrw_ss()) [cndbsuc_dV_behaviour] THEN 
+      ASM_SIMP_TAC (bsrw_ss()) [cndbsuc_dV_behaviour] THEN
       ASM_SIMP_TAC (srw_ss()) [Once numdB_def],
 
-      `0 < N` by SRW_TAC [][Abbr`N`] THEN 
-      `N DIV 3 < N` 
-        by SRW_TAC [ARITH_ss][arithmeticTheory.DIV_LESS] THEN 
-      `N DIV 3 ≤ c` by SRW_TAC [ARITH_ss][Abbr`N`] THEN 
+      `0 < N` by SRW_TAC [][Abbr`N`] THEN
+      `N DIV 3 < N`
+        by SRW_TAC [ARITH_ss][arithmeticTheory.DIV_LESS] THEN
+      `N DIV 3 ≤ c` by SRW_TAC [ARITH_ss][Abbr`N`] THEN
       Cases_on `N MOD 3 = 1` THENL [
-        ASM_SIMP_TAC (bsrw_ss()) [cndbsuc_dAPP_behaviour, Once numdB_def] THEN 
+        ASM_SIMP_TAC (bsrw_ss()) [cndbsuc_dAPP_behaviour, Once numdB_def] THEN
         `nsnd (N DIV 3) ≤ c ∧ nfst (N DIV 3) ≤ c`
-           by (ASSUME_TAC (Q.INST [`n` |-> `N DIV 3`] 
+           by (ASSUME_TAC (Q.INST [`n` |-> `N DIV 3`]
                                   numpairTheory.nsnd_le) THEN
-               ASSUME_TAC (Q.INST [`n` |-> `N DIV 3`] 
+               ASSUME_TAC (Q.INST [`n` |-> `N DIV 3`]
                                   numpairTheory.nfst_le) THEN
-               DECIDE_TAC) THEN 
-        ASM_SIMP_TAC (bsrw_ss()) [cnfst_behaviour, cnsnd_behaviour, 
+               DECIDE_TAC) THEN
+        ASM_SIMP_TAC (bsrw_ss()) [cnfst_behaviour, cnsnd_behaviour,
                                   cdAPP_behaviour],
 
-        ASM_SIMP_TAC (bsrw_ss()) [cndbsuc_dABS_behaviour, Once numdB_def, 
+        ASM_SIMP_TAC (bsrw_ss()) [cndbsuc_dABS_behaviour, Once numdB_def,
                                   cdABS_behaviour]
       ]
     ],
 
-    ASM_SIMP_TAC (bsrw_ss()) [cB_behaviour] THEN 
-    `n ≤ c` by SRW_TAC [ARITH_ss][Abbr`N`] THEN 
+    ASM_SIMP_TAC (bsrw_ss()) [cB_behaviour] THEN
+    `n ≤ c` by SRW_TAC [ARITH_ss][Abbr`N`] THEN
     ASM_SIMP_TAC (bsrw_ss()) []
   ]);
 
 val cnumdB_def = Define`
   cnumdB = LAM "n" (cnumdB0 @@ VAR "n" @@ VAR "n")
-`; 
+`;
 
 val FV_cnumdB = Store_thm(
   "FV_cnumdB",
@@ -1085,5 +1085,59 @@ val cnumdB_behaviour = store_thm(
   "cnumdB_behaviour",
   ``cnumdB @@ church n -n->* cDB (numdB n)``,
   SIMP_TAC (bsrw_ss()) [cnumdB_def, cnumdB0_behaviour]);
-  
+
+(* ----------------------------------------------------------------------
+    Computable version of bnf_of, bringing us pretty well all the way to
+    a universal machine
+   ---------------------------------------------------------------------- *)
+
+val cbnfof_body_def = Define`
+  cbnfof_body =
+  LAM "f" (LAM "t" (cbnf @@ VAR "t"
+                         @@ VAR "t"
+                         @@ (VAR "f" @@ (cnoreduct @@ VAR "t"))))
+`;
+
+val cbnfof_body_equiv0 = brackabs_equiv [] cbnfof_body_def
+val cbnfof_body_equiv = brackabs_equiv [B_I_uncond] cbnfof_body_equiv0
+
+val FV_cbnfof_body = Store_thm(
+  "FV_cbnfof_body",
+  ``FV cbnfof_body = {}``,
+  SRW_TAC [][cbnfof_body_def, EXTENSION]);
+
+val _ = reveal "Y"
+
+val cbnf_of_def = Define`cbnf_of = Y @@ cbnfof_body`
+val FV_cbnf = Store_thm(
+  "FV_cbnf",
+  ``FV cbnf_of = {}``,
+  SRW_TAC [][cbnf_of_def]);
+
+val cbnf_of_lemma = prove(
+  ``∀t. (OWHILE ((~) o bnf) (THE o noreduct) t0 = SOME t) ⇒
+        Y @@ cbnfof_body @@ cDB (fromTerm t0) ==
+          Y @@ cbnfof_body @@ cDB (fromTerm t)``,
+  HO_MATCH_MP_TAC whileTheory.OWHILE_INV_IND THEN SRW_TAC [][] THEN
+  ASM_SIMP_TAC (bsrw_ss()) [] THEN
+  ASM_SIMP_TAC (bsrw_ss()) [Once chap2Theory.lameq_Y] THEN
+  ASM_SIMP_TAC (bsrw_ss()) [cbnfof_body_equiv, cbnf_behaviour,
+                            cnoreduct_behaviour, cB_behaviour]);
+
+val cbnf_of_works1 = store_thm(
+  "cbnf_of_works1",
+  ``(bnf_of M = SOME N) ⇒
+    cbnf_of @@ cDB (fromTerm M) -n->* cDB (fromTerm N)``,
+  SRW_TAC [][cbnf_of_def, bnf_of_def] THEN
+  IMP_RES_TAC cbnf_of_lemma THEN
+  ASM_SIMP_TAC (bsrw_ss()) [] THEN
+  ASM_SIMP_TAC (bsrw_ss()) [Once chap2Theory.lameq_Y] THEN
+  IMP_RES_TAC whileTheory.OWHILE_ENDCOND THEN
+  FULL_SIMP_TAC (srw_ss()) [] THEN
+  ASM_SIMP_TAC (bsrw_ss()) [cbnfof_body_equiv, cB_behaviour,
+                            cbnf_behaviour]);
+
+(* proving the other direction will be a pain *)
+
+
 val _ = export_theory()
